src/lib/kernels/Kuiper.HReduceU32Plus.fsti
@@ -9,14 +9,14 @@ open Kuiper.Seq.Common
 open Kuiper.IsReduction
 
 module SZ = FStar.SizeT
-module U32 = FStar.UInt32
+module F = FStar.UInt32
 
 let size : sz = 1024sz
 
 (* no polymorphism, but at least keep the definitions here *)
-let ety = u32
-inline_for_extraction noextract let op  : ety -> ety -> ety = U32.add_mod
-inline_for_extraction noextract let neu : ety = U32.zero
+let ety = F.t
+inline_for_extraction noextract let op  : ety -> ety -> ety = F.add_mod
+inline_for_extraction noextract let neu : ety = F.zero
 
 (* Ownership of array r between i and j. The first value of that slice
 is the reduction of all the values in the (original) slice v. *)
@@ -32,8 +32,9 @@ let gpu_pts_to_slice_sum_inner
   ** pure (i < j /\ j <= sz /\
            len v = sz /\
            len s = j - i /\
-           squash (is_reduction neu op (Seq.slice v i j) (Seq.index s 0))) // SQUASH VERY IMPORTANT!!
+           squash (is_reduction neu op (Seq.slice v i j) (s @! 0))) // SQUASH VERY IMPORTANT!!
 
+(* Not easy to mark this unfold as it has a lambda (in the exists) *)
 let gpu_pts_to_slice_sum
   (#sz:nat)
   ([@@@mkey] r: gpu_array ety sz)
@@ -62,23 +63,23 @@ let kpost (nth: nat) (a : gpu_array ety nth) (s : erased (seq ety))
 
 [@@ CPrologue "__device__"]
 inline_for_extraction
-fn reduce
+fn d_reduce
   (nth : sz { 0 < SZ.v nth /\ SZ.v nth <= 1024 })
   (a : gpu_array ety nth)
   (#s :  erased (seq ety))
   (#_: squash (len s == nth))
-  (etid : erased tid_t { (gdim_x etid <: nat) == 1ul /\ (bdim_x etid <: nat) == SZ.sizet_to_uint32 nth })
+  (etid : tid_t { (gdim_x etid <: nat) == 1ul /\ (bdim_x etid <: nat) == SZ.sizet_to_uint32 nth })
+  preserves
+    gpu ** thread_id etid
   requires
-    gpu **
-    thread_id etid **
     mbarrier_tok nth (barrier_matrix nth a s) 0 (tidx_x etid) **
     kpre nth a s (thread_index etid)
-  ensures 
-    gpu **
-    thread_id etid **
-    (exists* it. mbarrier_tok nth (barrier_matrix nth a s) it (tidx_x etid)) **
-    kpost nth a s (thread_index etid)
+  ensures
+    exists* it.
+      mbarrier_tok nth (barrier_matrix nth a s) it (tidx_x etid) **
+      kpost nth a s (thread_index etid)
 
+(* NB: cannot use 'preserves' as we depend on the shape of pre/post *)
 [@@ CPrologue "__global__"]
 inline_for_extraction
 fn k_reduce
@@ -86,7 +87,7 @@ fn k_reduce
   (a : gpu_array ety nth)
   (#s :  erased (seq ety))
   (#_: squash (len s == nth))
-  (etid : erased tid_t { (gdim_x etid <: nat) == 1ul /\ (bdim_x etid <: nat) == SZ.sizet_to_uint32 nth })
+  (etid : tid_t { (gdim_x etid <: nat) == 1ul /\ (bdim_x etid <: nat) == SZ.sizet_to_uint32 nth })
   requires
     gpu **
     thread_id etid **
@@ -97,3 +98,13 @@ fn k_reduce
     thread_id etid **
     (exists* it. mbarrier_tok nth (barrier_matrix nth a s) it (tidx_x etid)) **
     kpost nth a s (thread_index etid)
+
+fn reduce
+  (lena : szp { lena < max_threads })
+  (a : gpu_array ety lena)
+  requires
+    cpu **
+    gpu_pts_to_array a 'va
+  ensures
+    cpu **
+    (exists* va'. gpu_pts_to_array a va') (* underspec *)
